More work on Imp.

handouts/imp.v
@@ -35,6 +35,9 @@ Inductive com :=
 (* Run [c] while [e] is non-zero *)
 | While (e : expr) (c : com).
 
+
+
+
 (** We will start using several features of Rocq and stdpp more freely.  Rocq
     has a type class mechanism similar to that of Haskell, which allows us to
     overload operations.  The [EqDecision] type class says that a type has a
@@ -50,9 +53,16 @@ Proof. solve_decision. Defined.
 Global Instance com_eqdec : EqDecision com.
 Proof. solve_decision. Defined.
 
+
+
+
 (** We will now define several functions for evaluating programs of our
     language. First, we define a function [eval_binop] that applies a binary
-    operation to two numbers. *)
+    operation to two numbers.
+
+    ([bool_decide P] is an stdpp function that returns [true] if and only if [P]
+    holds.  It only works for propositions that were shown to be decidable, like
+    we did for equality on [com].) *)
 
 Definition eval_binop b :=
   match b with
@@ -68,6 +78,9 @@ Definition eval_binop b :=
     in Java or dictionaries in Python.  *)
 
 Definition state : Type := gmap string nat.
+
+
+
 
 (** We have several options to define the semantics.  The most traditional
     choice in Rocq is to define a reduction relation on states; for example,
@@ -107,28 +120,22 @@ Global Instance mbind_result : MBind result := fun A B f x =>
   | NotYet => NotYet
   end.
 
+
+
+
 (** We are now ready to evaluate expressions.  Note that the computation returns
     error if some variable is not defined in the current state [s]. *)
 
 Fixpoint eval_expr (e : expr) (s : state) : result nat :=
-  match e with
-  | Var x => if s !! x is Some n then Done n else Error
-  | Num n => Done n
-  | Binop b e1 e2 =>
-      n1 ← eval_expr e1 s;
-      n2 ← eval_expr e2 s;
-      Done (eval_binop b n1 n2)
-  end.
+NotYet.
+
+
 
 (** Evaluating an expression always yields a final result or an error. *)
 
 Lemma eval_expr_notyet e s : eval_expr e s ≠ NotYet.
-Proof.
-induction e as [x|n|b e1 IH1 e2 IH2]; rewrite /=; eauto.
-- destruct (s !! x); eauto.
-- destruct (eval_expr e1) as [r1| | ]; try done.
-  destruct (eval_expr e2) as [r2| | ]; done.
-Qed.
+Proof. Admitted.
+
 
 (** Ideally, to evaluate commands, we would write a function [eval_com] of type
     [com -> state -> result state].  Unfortunately, Rocq will not allow us to do
@@ -140,42 +147,35 @@ Qed.
     input [k] to the evaluation function, which counts the maximum number of
     iterations of [while] that we are allowed to perform. *)
 
-Fixpoint iter {T} (f : (T -> result T) -> T -> result T) (x : T) (k : nat)
-    : result T :=
+Fixpoint iter {T} (f : (T -> result T) -> T -> result T) k x : result T :=
   f (fun x' =>
       match k with
       | 0 => NotYet
-      | S k' => iter f x' k'
+      | S k' => iter f k' x'
       end) x.
 
-Fixpoint eval_com (c : com) (s : state) (k : nat) : result state :=
+Fixpoint eval_com (c : com) (k : nat) (s : state) : result state :=
   match c with
   | Skip =>
       Done s
 
   | Seq c1 c2 =>
-      s' ← eval_com c1 s k;
-      eval_com c2 s' k
+      s' ← eval_com c1 k s;
+      eval_com c2 k s'
 
   | Assign x e =>
       n ← eval_expr e s;
       Done (<[x := n]> s)
 
   | If e c1 c2 =>
-      n ← eval_expr e s;
-      if bool_decide (n = 0) then eval_com c2 s k
-      else eval_com c1 s k
+      NotYet
+      
+
 
   | While e c =>
-      let f eval_while s' : result state :=
-        n ← eval_expr e s';
-        if bool_decide (n = 0) then
-          Done s'
-        else
-          s'' ← eval_com c s' k;
-          eval_while s''
-      in
-      iter f s k
+      NotYet
+      
+
 
   end.
 
@@ -185,18 +185,19 @@ Fixpoint eval_com (c : com) (s : state) (k : nat) : result state :=
 
 Lemma result_done_mbind :
   forall {T S} (x : T) (f : T -> result S), mbind f (Done x) = f x.
-Proof. eauto. Qed.
+Proof. Admitted.
+
 
 Lemma result_mbind_done : forall {T} (x : result T), mbind Done x = x.
-Proof.
-intros T []; eauto.
-Qed.
+Proof. Admitted.
+
 
 Lemma result_mbind_assoc :
   forall {T S R} (g : S -> result R) (f : T -> result S) (x : result T),
     mbind g (mbind f x) =
     mbind (fun y : T => mbind g (f y)) x.
-Proof. intros T S R f g []; eauto. Qed.
+Proof. Admitted.
+
 
 (** If [mbind] returns [Done], then the computation must have succeeded in both
     stages. *)
@@ -205,7 +206,8 @@ Lemma result_mbind_inv :
   forall {T S} {f : T -> result S} {x : result T} {y : S},
     mbind f x = Done y ->
     exists a, x = Done a /\ f a = Done y.
-Proof. intros T S f [x | |] y; eauto; done. Qed.
+Proof. Admitted.
+
 
 (** We define an ordering relation on [result] as follows.  We say that [x] is
     _less defined_ than [y], written [x ⊑ y], if they are equal or [x] is
@@ -238,11 +240,8 @@ Lemma result_bind_mono :
     x ⊑ y ->
     (forall a, f a ⊑ g a) ->
     mbind f x ⊑ mbind g y.
-Proof.
-intros T S f g x y [H|H] f_g.
-- rewrite H. eauto.
-- rewrite H. destruct y as [a| |]; eauto.
-Qed.
+Proof. Admitted.
+
 
 (** (As an aside, this type of statement is common in frameworks for _relational
     reasoning_ about programs: being able to relate the final results of two
@@ -261,7 +260,7 @@ Lemma iter_mono :
       (forall x, f' x ⊑ g' x) ->
       (forall x, f f' x ⊑ g g' x)) ->
     n <= m ->
-    iter f x n ⊑ iter g x m.
+    iter f n x ⊑ iter g m x.
 Proof.
 intros T f g n m x f_g n_m.
 induction m as [|m IH] in n, n_m, x |- *.
@@ -276,20 +275,9 @@ Qed.
     results with more iterations. *)
 
 Lemma eval_com_mono :
-  forall n m c s, n <= m -> eval_com c s n ⊑ eval_com c s m.
-Proof.
-intros n m c s n_m.
-induction c as [|c1 IH1 c2 IH2|x e|e c1 IH1 c2 IH2|e c IH] in s |- *;
-  rewrite /=; eauto.
-- apply result_bind_mono; eauto.
-- apply result_bind_mono; eauto.
-  intros a. destruct (bool_decide _); eauto.
-- apply iter_mono; eauto.
-  intros f g f_g s'.
-  apply result_bind_mono; eauto.
-  intros a. destruct (bool_decide _); eauto.
-  apply result_bind_mono; eauto.
-Qed.
+  forall n m c s, n <= m -> eval_com c n s ⊑ eval_com c m s.
+Proof. Admitted.
+
 
 (** So much for definedness.  We are now going to reason about program safety.
     Usually, obtaining an error as the result of evaluation indicates that there
@@ -318,32 +306,11 @@ Fixpoint vars_com c : gset string :=
 
 (** Here is what we hope to prove: *)
 
-Lemma vars_com_not_error c s k :
+Lemma vars_com_not_error c k s :
   subseteq (vars_com c) (dom s) ->
-  eval_com c s k <> Error.
-Proof.
-induction c as [|c1 IH1 c2 IH2|x e|e c1 IH1 c2 IH2|e c IH] in s |- *;
-  rewrite /=.
-- done.
-- intros Hdom.
-  assert (subseteq (vars_com c1) (dom s) /\
-          subseteq (vars_com c2) (dom s)) as [H1 H2].
-  { rewrite -union_subseteq. done. }
-  assert (IH1' := IH1 _ H1).
-  destruct (eval_com c1 s k) as [s' | | ]; rewrite /=.
-  + apply IH2. (* Stuck... *)
-Abort.
+  eval_com c k s <> Error.
+Proof. Admitted.
 
-Lemma iter_ind :
-  forall {T} (P : result T -> Prop) (f : (T -> result T) -> T -> result T),
-    P NotYet ->
-    (forall f',
-      (forall x, P (Done x) -> P (f' x)) ->
-      (forall x, P (Done x) -> P (f f' x))) ->
-    forall x n, P (Done x) -> P (iter f x n).
-Proof.
-intros T P f H0 H1 x n Hx.
-induction n as [|n IH] in x, Hx |- *; rewrite /=.
-- apply H1; eauto.
-- apply H1; eauto.
-Qed.
+
+
+
